src/ComputableGraph.v
@@ -1,0 +1,128 @@
+From coqutil Require Import Map.Interface.
+From Stdlib Require Import List Bool.
+From DatalogRocq Require Import Graph.
+Import ListNotations.
+Import BoolNotations.
+
+Section ComputableGraph.
+Context {Node : Type}.
+Context {node_eqb : Node -> Node -> bool}.
+Context {node_eqb_spec : forall x y, BoolSpec (x = y) (x <> y) (node_eqb x y)}.
+Context {node_set : map.map Node unit}.
+Context {node_set_ok : map.ok node_set}.
+Context {edge_set : map.map Node node_set}.
+Context {edge_set_ok : map.ok edge_set}.
+
+Record ComputableGraph := {
+  nodes : node_set;
+  edges : edge_set
+}.
+
+Definition check_node_valid (n : Node) (ns : node_set) : bool :=
+  match map.get ns n with
+  | Some _ => true
+  | None => false
+  end.
+
+Definition check_edge_valid (n1 n2 : Node) (ns : node_set) : bool :=
+  check_node_valid n1 ns && check_node_valid n2 ns.
+
+(* Check all edges only use nodes from the node set *)
+Definition check_edges_valid (es : edge_set) (ns : node_set) : bool :=
+  map.forallb (fun n1 neighbors =>
+    map.forallb (fun n2 _ =>
+      check_edge_valid n1 n2 ns
+    ) neighbors
+  ) es.
+
+Definition check_graph_valid (cg : ComputableGraph) : bool :=
+  check_edges_valid cg.(edges) cg.(nodes).
+
+Definition cg_nodes_to_g_nodes (ns : node_set) : Node -> Prop :=
+  fun n => check_node_valid n ns = true.
+
+Definition check_edge_exists (n1 n2 : Node) (es : edge_set) : bool :=
+  match map.get es n1 with
+  | Some neighbors => match map.get neighbors n2 with
+                      | Some _ => true
+                      | None => false
+                      end
+  | None => false
+  end.
+
+Definition cg_edges_to_g_edges (es : edge_set) (ns : node_set) : Node -> Node -> Prop :=
+  fun n1 n2 => check_edge_exists n1 n2 es = true.
+
+Definition computable_graph_to_graph (cg : ComputableGraph) : Graph :=
+  {|
+    Graph.nodes := fun n => check_node_valid n cg.(nodes) = true;
+    Graph.edge := fun n1 n2 => check_edge_exists n1 n2 cg.(edges) = true
+  |}.
+
+Lemma forallb_spec : forall {key val : Type} {m : map.map key val} {ok : map.ok m}
+    (key_eq_dec : forall k1 k2 : key, {k1 = k2} + {k1 <> k2})
+    (f : key -> val -> bool) (mp : m),
+  map.forallb f mp = true <->
+  forall k v, map.get mp k = Some v -> f k v = true.
+Proof.
+  intros. unfold map.forallb.
+  eapply (map.fold_spec (fun mp r => r = true <-> forall k v, map.get mp k = Some v -> f k v = true)).
+  - split.
+    + intros _ k v. rewrite map.get_empty. discriminate.
+    + intros. reflexivity.
+  - intros k v m' r Hget [IHf IHb].
+    split.
+    + intros Handb k' v' Hget'.
+      apply andb_prop in Handb. destruct Handb as [Hr Hf].
+      destruct (key_eq_dec k' k) as [->|Hne].
+      * rewrite map.get_put_same in Hget'. inversion Hget'. subst. exact Hf.
+      * rewrite map.get_put_diff in Hget' by exact Hne.
+        exact (IHf Hr k' v' Hget').
+    + intros Hall.
+      apply andb_true_intro. split.
+      * apply IHb. intros k' v' Hget'.
+        apply Hall. rewrite map.get_put_diff; [exact Hget'|].
+        intros ->. rewrite Hget in Hget'. discriminate.
+      * apply Hall. rewrite map.get_put_same. reflexivity.
+Qed.
+
+Definition node_eq_dec : forall n1 n2 : Node, {n1 = n2} + {n1 <> n2}.
+Proof.
+  intros n1 n2.
+  case_eq (node_eqb n1 n2); intro Heq.
+  - left. destruct (node_eqb_spec n1 n2); auto; discriminate.
+  - right. destruct (node_eqb_spec n1 n2); auto; discriminate.
+Qed.
+
+Lemma check_graph_correct : forall cg,
+  check_graph_valid cg = true <-> good_graph (computable_graph_to_graph cg).
+Proof.
+  intros cg.
+  unfold check_graph_valid, check_edges_valid, good_graph, computable_graph_to_graph. simpl.
+  unfold check_edges_valid.
+  rewrite (forallb_spec node_eq_dec).
+  split.
+  - intros H n1 n2 Hedge.
+    (* Hedge : check_edge_exists n1 n2 cg.(edges) = true *)
+    unfold check_edge_exists in Hedge.
+    destruct (map.get cg.(edges) n1) eqn:E1; try discriminate.
+    destruct (map.get r n2) eqn:E2; try discriminate.
+    specialize (H n1 r E1).
+    rewrite (forallb_spec node_eq_dec) in H.
+    specialize (H n2 u E2).
+    unfold check_edge_valid in H.
+    apply andb_prop in H. destruct H as [Hn1 Hn2].
+    split; assumption.
+  - intros H n1 neighbors Hn1.
+    rewrite (forallb_spec node_eq_dec).
+    intros n2 u Hn2.
+    unfold check_edge_valid.
+    apply andb_true_intro.
+    assert (Hedge : check_edge_exists n1 n2 cg.(edges) = true).
+    { unfold check_edge_exists. rewrite Hn1, Hn2. reflexivity. }
+    apply H in Hedge.
+    destruct Hedge as [Hn1valid Hn2valid].
+    split; assumption.
+Qed.
+
+End ComputableGraph.
