src/Examples/Programs/PrintPrograms.v
@@ -5,7 +5,7 @@ Print Printer.
 
 Redirect "json_examples/basic_program" Eval compute in (to_string (encode basic_program)).
 Redirect "json_examples/family_program" Eval compute in (to_string (encode family_program)).
-Redirect "json_examples/graph_program" Eval compute in (to_string (encode graph_program)).
+(* Redirect "json_examples/graph_program" Eval compute in (to_string (encode graph_program)). *)
 Redirect "json_examples/netkat_program" Eval compute in (to_string (encode netkat_program)).
 
 Instance JEncode_Bfn : JEncode Bfn :=
