src/Graph.v
@@ -1,0 +1,27 @@
+Section Graph.
+  
+  Context {Node : Type}.
+  Context {node_eqb : Node -> Node -> bool}.
+  Context {node_eqb_spec : forall x y, BoolSpec (x = y) (x <> y) (node_eqb x y)}.
+
+  Record Graph := {
+    nodes : Node -> Prop;
+    edge : Node -> Node -> Prop
+  }.
+
+  Definition good_graph (g : Graph) := 
+   forall n1 n2, edge g n1 n2 -> nodes g n1 /\ nodes g n2.
+
+  Inductive path (g : Graph) : Node -> Node -> Prop :=
+  | path_nil n :
+      g.(nodes) n ->
+      path g n n 
+  | path_cons n1 n2 n3 :
+      g.(edge) n1 n2 ->
+      path g n2 n3 ->
+      path g n1 n3.
+
+  Definition strongly_connected (g : Graph) : Prop :=
+    forall n1 n2, g.(nodes) n1 -> g.(nodes) n2 -> path g n1 n2.
+    
+End Graph.
