Makefile
@@ -1,12 +1,14 @@
 COQMAKEFILE ?= Makefile.coq
 
 all: $(COQMAKEFILE)
+	mkdir -p output
 	$(MAKE) -f $(COQMAKEFILE)
 
 $(COQMAKEFILE): _CoqProject
 	coq_makefile -f _CoqProject -o $(COQMAKEFILE)
 
 clean: $(COQMAKEFILE)
+	rm -rf output
 	$(MAKE) -f $(COQMAKEFILE) clean
 	rm -f $(COQMAKEFILE) $(COQMAKEFILE).conf
 	find . -type f \( -name '*~' -o -name '*.aux' -o -name '.lia.cache' -o -name '.nia.cache' \) -delete
